cvc5.lean
@@ -325,34 +325,6 @@ end Result
 
 
 
-private opaque ProofImpl : NonemptyType.{0}
-
-/-- A cvc5 proof.
-
-Proofs are trees and every proof object corresponds to the root step of a proof. The branches of the
-root step are the premises of the step.
--/
-@[irreducible]
-def Proof : (ω : Type) → Type := fun _ => ProofImpl.type
-
-namespace Proof
-
-private theorem typeDef : Proof ω = ProofImpl.type :=
-  by unfold Proof ; rfl
-
-private def toImpl : Proof ω → ProofImpl.type :=
-  by rw [typeDef] ; exact id
-
-private def ofImpl : ProofImpl.type → Proof ω :=
-  by rw [typeDef] ; exact id
-
-instance instNonemptyProof : Nonempty (Proof ω) :=
-  by rw [typeDef] ; exact ProofImpl.property
-
-end Proof
-
-
-
 /-! ## FFI constructor
 
 The following constructors are only used by C++ to inject values as `Except Error _`.
@@ -411,8 +383,6 @@ structure Env (ω : Type) (α : Type) where
 private ofRaw ::
   toRaw : ReaderT Cvc5.TermManager (ExceptT Error BaseIO) α
 
-namespace Env
-
 def run (code : {ω : Type} → Env ω α) : ExceptT Error BaseIO α := do
   let tm ← TermManager.new ()
   (@code Unit).toRaw tm
@@ -421,6 +391,8 @@ def runIO (code : {ω : Type} → Env ω α) : IO α := fun world =>
   match run code world with
   | .ok (.ok res) world => .ok res world
   | .ok (.error err) world => .error err.toIO world
+
+namespace Env
 
 instance : Monad (Env ω) where
   pure := (⟨pure ·⟩)
@@ -488,6 +460,8 @@ protected extern_def toString : Srt ω → String
 
 instance : ToString (Srt ω) := ⟨Srt.toString⟩
 
+instance : Repr (Srt ω) := ⟨fun self _ => self.toString⟩
+
 /-- Comparison for structural equality. -/
 protected extern_def beq : Srt ω → Srt ω → Bool
 
@@ -529,6 +503,467 @@ instance : DecidableLE (Srt ω) :=
 protected extern_def hash : Srt ω → UInt64
 
 instance : Hashable (Srt ω) := ⟨Srt.hash⟩
+
+end Srt
+
+
+
+private opaque TermImpl : NonemptyType.{0}
+
+/-- A cvc5 term. -/
+@[irreducible]
+def Term : (ω : Type) → Type := fun _ => TermImpl.type
+
+namespace Term
+
+private theorem typeDef : Term ω = TermImpl.type :=
+  by unfold Term ; rfl
+
+private def toImpl : Term ω → TermImpl.type :=
+  by rw [typeDef] ; exact id
+
+private def ofImpl : TermImpl.type → Term ω :=
+  by rw [typeDef] ; exact id
+
+instance instNonemptyTerm : Nonempty (Term ω) :=
+  by rw [typeDef] ; exact TermImpl.property
+
+private extern_def null : Unit → Term ω
+
+instance : Inhabited (Term ω) := ⟨null ()⟩
+
+/-- A string representation of this term. -/
+protected extern_def toString : Term ω → String
+
+instance : ToString (Term ω) := ⟨Term.toString⟩
+
+/-- Syntactic equality operator. -/
+protected extern_def beq : (Term ω) → (Term ω) → Bool
+
+instance : BEq (Term ω) := ⟨Term.beq⟩
+
+protected extern_def hash : (Term ω) → UInt64
+
+instance : Hashable (Term ω) := ⟨Term.hash⟩
+
+/-- Determine if this term is nullary. -/
+extern_def isNull : Term ω → Bool
+
+end Term
+
+
+
+private opaque OpImpl : NonemptyType.{0}
+
+/-- A cvc5 term. -/
+@[irreducible]
+def Op : (ω : Type) → Type := fun _ => OpImpl.type
+
+namespace Op
+
+private theorem typeDef : Op ω = OpImpl.type :=
+  by unfold Op ; rfl
+
+private def toImpl : Op ω → OpImpl.type :=
+  by rw [typeDef] ; exact id
+
+private def ofImpl : OpImpl.type → Op ω :=
+  by rw [typeDef] ; exact id
+
+instance instNonemptyOp : Nonempty (Op ω) :=
+  by rw [typeDef] ; exact OpImpl.property
+
+@[extern "term_null"]
+private opaque null : Unit → Op ω
+
+instance : Inhabited (Op ω) := ⟨null ()⟩
+
+/-- A string representation of this term. -/
+protected extern_def toString : Op ω → String
+
+instance : ToString (Op ω) := ⟨Op.toString⟩
+
+end Op
+
+
+
+private opaque ProofImpl : NonemptyType.{0}
+
+/-- A cvc5 proof.
+
+Proofs are trees and every proof object corresponds to the root step of a proof. The branches of the
+root step are the premises of the step.
+-/
+@[irreducible]
+def Proof : (ω : Type) → Type := fun _ => ProofImpl.type
+
+namespace Proof
+
+private theorem typeDef : Proof ω = ProofImpl.type :=
+  by unfold Proof ; rfl
+
+private def toImpl : Proof ω → ProofImpl.type :=
+  by rw [typeDef] ; exact id
+
+private def ofImpl : ProofImpl.type → Proof ω :=
+  by rw [typeDef] ; exact id
+
+instance instNonemptyProof : Nonempty (Proof ω) :=
+  by rw [typeDef] ; exact ProofImpl.property
+
+/-- The null proof. -/
+extern_def null : Unit → Proof ω
+
+instance : Inhabited (Proof ω) := ⟨null ()⟩
+
+end Proof
+
+
+
+private opaque SolverImpl : NonemptyType.{0}
+
+/-- A cvc5 solver. -/
+private def Solver.Raw : Type := SolverImpl.type
+
+namespace Solver.Raw
+
+instance : Nonempty Solver.Raw := SolverImpl.property
+
+end Solver.Raw
+
+structure Solver (ω : Type) where
+private mk' ::
+  /-- Underlying raw solver. -/
+  private toRaw : Solver.Raw
+  /-- Parser placeholder. -/
+  private parser : IO.Ref (Option Unit)
+
+namespace Solver
+
+/-- Constructor.
+
+Constructs solver instance from a given term manager instance.
+
+- `tm`: The associated term manager.
+-/
+@[extern "solver_new"]
+private opaque Raw.new : TermManager → Solver.Raw
+
+private def ofManager (tm : TermManager) : BaseIO (Solver ω) := do
+  let parser ← IO.mkRef none
+  return {toRaw := Raw.new tm, parser}
+
+def new : Env ω (Solver ω) := Env.managerDo (liftM ∘ ofManager)
+
+section variable (solver : Solver ω)
+
+private def rawSolverDo (f : Solver.Raw → Env ω α) : Env ω α :=
+  f solver.toRaw
+
+private def rawSolverDo? (f : Solver.Raw → Except Error α) : Env ω α :=
+  solver.rawSolverDo (liftM ∘ f)
+
+end
+
+end Solver
+
+
+
+/-! ## User-facing definitions -/
+
+
+
+namespace TermManager
+
+/-- Get the Boolean sort. -/
+private extern_def getBooleanSort : TermManager → Srt ω
+
+/-- Get the Integer sort. -/
+private extern_def getIntegerSort : TermManager → Srt ω
+
+/-- Get the Real sort. -/
+private extern_def getRealSort : TermManager → Srt ω
+
+/-- Get the regular expression sort. -/
+private extern_def getRegExpSort : TermManager → Srt ω
+
+/-- Get the rounding mode sort. -/
+private extern_def getRoundingModeSort : TermManager → Srt ω
+
+/-- Get the string sort. -/
+private extern_def getStringSort : TermManager → Srt ω
+
+/-- Create an array sort.
+
+- `indexSort` The array index sort.
+- `elemSort` The array element sort.
+-/
+extern_def!? mkArraySort : TermManager → (indexSort elemSort : Srt ω) → Except Error (Srt ω)
+
+/-- Create a bit-vector sort.
+
+- `size` The bit-width of the bit-vector sort.
+-/
+extern_def!? mkBitVectorSort : TermManager → (size : UInt32) → Except Error (Srt ω)
+
+/-- Create a floating-point sort.
+
+- `exp` The bit-width of the exponent of the floating-point sort.
+- `sig` The bit-width of the significand of the floating-point sort.
+-/
+extern_def!? mkFloatingPointSort : TermManager → (exp sig : UInt32) → Except Error (Srt ω)
+
+/-- Create a finite-field sort from a given string of base n.
+
+- `size` The modulus of the field. Must be a prime.
+-/
+private extern_def mkFiniteFieldSortFromString
+: TermManager → (size : String) → (base : UInt32 := 10) → Except Error (Srt ω)
+
+@[inherit_doc mkFiniteFieldSortFromString]
+abbrev mkFiniteFieldSort (tm : TermManager) : (size : Nat) → Except Error (Srt ω) :=
+  (tm.mkFiniteFieldSortFromString · 10) ∘ toString
+@[inherit_doc mkFiniteFieldSortFromString]
+abbrev mkFiniteFieldSort! (tm : TermManager) : (size : Nat) → Srt ω :=
+  Error.unwrap! ∘ (tm.mkFiniteFieldSortFromString · 10) ∘ toString
+@[inherit_doc mkFiniteFieldSortFromString]
+abbrev mkFiniteFieldSort? (tm : TermManager) : (size : Nat) → Option (Srt ω) :=
+  Except.toOption ∘ (tm.mkFiniteFieldSortFromString · 10) ∘ toString
+
+/-- Create function sort.
+
+- `sorts` The sort of the function arguments.
+- `codomain` The sort of the function return value.
+-/
+extern_def!? mkFunctionSort
+: TermManager → (sorts : Array (Srt ω)) → (codomain : Srt ω) → Except Error (Srt ω)
+
+/-- Create a predicate sort.
+
+This is equivalent to calling `mkFunctionSort` with Boolean sort as the codomain.
+
+- `sorts` The list of sorts of the predicate.
+-/
+extern_def!? mkPredicateSort : TermManager → (sorts : Array (Srt ω)) → Except Error (Srt ω)
+
+/-- Create a tuple sort.
+
+- `sorts` The sorts of the elements of the tuple.
+-/
+extern_def!? mkTupleSort : TermManager → (sorts : Array (Srt ω)) → Except Error (Srt ω)
+
+/-- Create an uninterpreted sort constructor sort.
+
+An uninterpreted sort constructor is an uninterpreted sort with arity > 0.
+
+- `arity` The arity of the sort (must be > 0).
+- `symbol` The symbol of the sort.
+-/
+extern_def!? mkUninterpretedSortConstructorSort
+: TermManager → (arity : Nat) → (symbol : String) → Except Error (Srt ω)
+
+/-- Create a set parameter.
+
+- `elemSort` The sort of the set elements.
+-/
+extern_def!? mkSetSort : TermManager → (sort : Srt ω) → Except Error (Srt ω)
+
+/-- Create a set parameter.
+
+- `elemSort` The sort of the set elements.
+-/
+extern_def!? mkBagSort : TermManager → (sort : Srt ω) → Except Error (Srt ω)
+
+/-- Create a set parameter.
+
+- `elemSort` The sort of the set elements.
+-/
+extern_def!? mkSequenceSort : TermManager → (sort : Srt ω) → Except Error (Srt ω)
+
+/-- Create an abstract sort. An abstract sort represents a sort for a given kind whose parameters
+and arguments are unspecified.
+
+The kind `k` must be the kind of a sort that can be abstracted, *i.e.* a sort that has indices or
+arguments sorts. For example, `SortKind.ARRAY_SORT` and `SortKind.BITVECTOR_SORT` can be passed as
+the kind `k` to this function, while `SortKind.INTEGER_SORT` and `SortKind.STRING_SORT` cannot.
+
+**NB:** Providing the kind `SortKind.ABSTRACT_SORT` as an argument to this function returns the
+(fully) unspecified sort, denoted `?`.
+
+**NB:** Providing a kind `k` that has no indices and a fixed arity of argument sorts will return the
+sort of kind `k` whose arguments are the unspecified sort. For example, `mkAbstractSort
+SortKind.ARRAY_SORT` will return the sort `(ARRAY_SORT ? ?)` instead of the abstract sort whose
+abstract kind is `SortKind.ARRAY_SORT`.
+-/
+extern_def!? mkAbstractSort : TermManager → (k : SortKind) → Except Error (Srt ω)
+
+/-- Create an uninterpreted sort.
+
+- `symbol` The name of the sort.
+-/
+extern_def mkUninterpretedSort : TermManager → (symbol : String) → (Srt ω)
+
+/-- Create a nullable sort.
+
+- `sort` The sort of the element of the nullable.
+-/
+extern_def!? mkNullableSort : TermManager → (sort : Srt ω) → Except Error (Srt ω)
+
+/-- Create a sort parameter.
+
+- `symbol` The name of the sort.
+
+**Warning**: This function is experimental and may change in future versions.
+-/
+extern_def mkParamSort : TermManager → (symbol : String) → Srt ω
+
+/-- Create a Boolean constant.
+
+- `b`: The Boolean constant.
+-/
+extern_def mkBoolean : TermManager → (b : Bool) → Term ω
+
+/-- Create an integer-value term.
+
+- `s`: the string representation of the constant, may represent an integer such as (`"123"`).
+-/
+private extern_def mkIntegerFromString : TermManager → (s : String) → Except Error (Term ω)
+with
+  /-- Create an integer-value term. -/
+  mkInteger (tm : TermManager) : Int → (Term ω) :=
+    Error.unwrap! ∘ tm.mkIntegerFromString ∘ toString
+
+/-- Create a real-value term.
+
+- `s`: the string representation of the constant, may represent an integer (`"123"`) or a real
+  constant (`"12.34"`, `"12/34"`).
+-/
+private extern_def mkRealFromString : TermManager → (s : String) → Except Error (Term ω)
+with
+  /-- Create a real-value term from a `Std.Internal.Rat`. -/
+  mkRealOfRat (tm : TermManager) (rat : Std.Internal.Rat) : Term ω :=
+    tm.mkRealFromString s!"{rat.num}/{rat.den}" |> Error.unwrap!
+  /-- Create a real-value term from numerator/denominator `Int`-s. -/
+  mkReal (tm : TermManager)
+    (num : Int) (den : Int := 1) (den_ne_0 : den ≠ 0 := by simp <;> omega)
+  : Term ω :=
+    let (num, den) :=
+      match h : den with
+      | .ofNat 0 => by contradiction
+      | .ofNat den => (num, den)
+      | .negSucc denMinus1 => (-num, denMinus1.succ)
+    mkRealOfRat tm <| Std.Internal.mkRat num den
+
+/-- Create operator of Kind:
+
+- `Kind.BITVECTOR_EXTRACT`
+- `Kind.BITVECTOR_REPEAT`
+- `Kind.BITVECTOR_ROTATE_LEFT`
+- `Kind.BITVECTOR_ROTATE_RIGHT`
+- `Kind.BITVECTOR_SIGN_EXTEND`
+- `Kind.BITVECTOR_ZERO_EXTEND`
+- `Kind.DIVISIBLE`
+- `Kind.FLOATINGPOINT_TO_FP_FROM_FP`
+- `Kind.FLOATINGPOINT_TO_FP_FROM_IEEE_BV`
+- `Kind.FLOATINGPOINT_TO_FP_FROM_REAL`
+- `Kind.FLOATINGPOINT_TO_FP_FROM_SBV`
+- `Kind.FLOATINGPOINT_TO_FP_FROM_UBV`
+- `Kind.FLOATINGPOINT_TO_SBV`
+- `Kind.FLOATINGPOINT_TO_UBV`
+- `Kind.INT_TO_BITVECTOR`
+- `Kind.TUPLE_PROJECT`
+
+See `cvc5.Kind` for a description of the parameters.
+
+- `kind` The kind of the operator.
+- `args` The arguments (indices) of the operator.
+
+If `args` is empty, the `Op` simply wraps the `cvc5.Kind`. The `Kind` can be used in
+`Solver.mkTerm` directly without creating an `Op` first.
+-/
+extern_def!? mkOpOfIndices
+: TermManager → (kind : Kind) → (args : Array Nat := #[]) → Except Error (Op ω)
+
+@[inherit_doc mkOpOfIndices]
+abbrev mkOp := @mkOpOfIndices
+@[inherit_doc mkOpOfIndices!]
+abbrev mkOp! := @mkOpOfIndices!
+@[inherit_doc mkOpOfIndices?]
+abbrev mkOp? := @mkOpOfIndices?
+
+/-- Create operator of kind:
+
+- `Kind.DIVISIBLE` (to support arbitrary precision integers)
+
+See `cvc5.Kind` for a description of the parameters.
+
+- `kind` The kind of the operator.
+- `arg` The string argument to this operator.
+-/
+extern_def!? mkOpOfString : TermManager → (kind : Kind) → (arg : String) → Except Error (Op ω)
+
+/-- Create n-ary term of given kind.
+
+- `kind` The kind of the term.
+- `children` The children of the term.
+-/
+extern_def!? mkTerm
+: TermManager → (kind : Kind) → (children : Array (Term ω) := #[]) → Except Error (Term ω)
+
+/-- Create n-ary term of given kind from a given operator.
+
+Create operators with `mkOp`.
+
+- `op` The operator.
+- `children` The children of the term.
+-/
+extern_def!? mkTermOfOp
+: TermManager → (op : Op ω) → (children : Array (Term ω) := #[]) → Except Error (Term ω)
+
+/-- Create a free constant.
+
+Note that the returned term is always fresh, even if the same arguments were provided on a
+previous call to `mkConst`.
+
+- `sort` The sort of the constant.
+- `symbol` The name of the constant (optional).
+-/
+private extern_def mkConst : TermManager → Srt ω → String → Term ω
+
+/--
+Create a bound variable to be used in a binder (i.e., a quantifier, a lambda, or a witness binder).
+
+The returned term is always fresh, even if the same arguments were provided on a previous call to
+mkConst().
+
+- `sort`: the sort of the variable.
+- `symbol`: the name of the variable (optional).
+-/
+extern_def mkVar : TermManager → Srt ω → String → Term ω
+
+end TermManager
+
+@[inherit_doc TermManager.getBooleanSort]
+def getBooleanSort : Env ω (Srt ω) := Env.managerDo (return TermManager.getBooleanSort ·)
+
+@[inherit_doc TermManager.getIntegerSort]
+def getIntegerSort : Env ω (Srt ω) := Env.managerDo (return TermManager.getIntegerSort ·)
+
+@[inherit_doc TermManager.getRealSort]
+def getRealSort : Env ω (Srt ω) := Env.managerDo (return TermManager.getRealSort ·)
+
+@[inherit_doc TermManager.getRegExpSort]
+def getRegExpSort : Env ω (Srt ω) := Env.managerDo (return TermManager.getRegExpSort ·)
+
+@[inherit_doc TermManager.getRoundingModeSort]
+def getRoundingModeSort : Env ω (Srt ω) := Env.managerDo (return TermManager.getRoundingModeSort ·)
+
+@[inherit_doc TermManager.getStringSort]
+def getStringSort : Env ω (Srt ω) := Env.managerDo (return TermManager.getStringSort ·)
+
+
+
+namespace Srt
 
 /-- Get the kind of this sort. -/
 extern_def getKind : Srt ω → SortKind
@@ -711,86 +1146,227 @@ Create sort parameters with `TermManager.mkParamSort symbol`.
 -/
 extern_def!? instantiate : Srt ω → (params : Array (Srt ω)) → Except Error (Srt ω)
 
+/-- Simultaneous substitution of Sorts.
+
+Note that this replacement is applied during a pre-order traversal and only once to the sort. It is not run until fix point. In the case that `sorts` contains duplicates, the replacement earliest in
+the vector takes priority.
+
+**Warning:** This function is experimental and may change in future versions.
+
+- `sorts` The sub-sorts to be substituted within this sort.
+- `replacements` The sort replacing the substituted sub-sorts.
+-/
+extern_def!? substitute
+: Srt ω → (sorts : Array (Srt ω)) → (replacements : Array (Srt ω)) → Except Error (Srt ω)
+
 end Srt
 
 
 
-private opaque TermImpl : NonemptyType.{0}
+namespace Op
 
-/-- A cvc5 term. -/
-@[irreducible]
-def Term : (ω : Type) → Type := fun _ => TermImpl.type
+/-- Syntactic equality operator. -/
+protected extern_def beq : Op ω → Op ω → Bool
+
+instance : BEq (Op ω) := ⟨Op.beq⟩
+
+/-- Get the kind of this operator. -/
+extern_def getKind : Op ω → Kind
+
+/-- Determine if this operator is nullary. -/
+extern_def isNull : Op ω → Bool
+
+/-- Determine if this operator is indexed. -/
+extern_def isIndexed : Op ω → Bool
+
+/-- Get the number of indices of this operator. -/
+extern_def getNumIndices : Op ω → Nat
+
+/-- Get the index at position `i` of an indexed operator. -/
+protected extern_def get : (op : Op ω) → Fin op.getNumIndices → Term ω
+
+instance : GetElem (Op ω) Nat (Term ω) fun op i => i < op.getNumIndices where
+  getElem op i h := op.get ⟨i, h⟩
+
+end Op
+
+
 
 namespace Term
 
-private theorem typeDef : Term ω = TermImpl.type :=
-  by unfold Term ; rfl
+/-- Get the kind of this term. -/
+extern_def getKind : Term ω → Kind
 
-private def toImpl : Term ω → TermImpl.type :=
-  by rw [typeDef] ; exact id
+/-- Get the sort of this term. -/
+extern_def getSort : Term ω → Srt ω
 
-private def ofImpl : TermImpl.type → Term ω :=
-  by rw [typeDef] ; exact id
+/-- Determine if this term has an operator. -/
+extern_def hasOp : Term ω → Bool
 
-instance instNonemptyTerm : Nonempty (Term ω) :=
-  by rw [typeDef] ; exact TermImpl.property
+/-- Determine if this term has a symbol (a name).
 
-@[extern "term_null"]
-private opaque null : Unit → Term ω
+For example, free constants and variables have symbols.
+-/
+extern_def hasSymbol : Term ω → Bool
 
-instance : Inhabited (Term ω) := ⟨null ()⟩
+/-- Get the id of this term. -/
+extern_def getId : Term ω → Nat
 
-/-- A string representation of this term. -/
-protected extern_def toString : Term ω → String
+/-- Get the number of children of this term. -/
+extern_def getNumChildren : Term ω → Nat
 
-instance : ToString (Term ω) := ⟨Term.toString⟩
+/-- Is this term a skolem? -/
+extern_def isSkolem : Term ω → Bool
+
+/-- Get the child term of this term at a given index. -/
+protected extern_def get : (t : Term ω) → Fin t.getNumChildren → Term ω
+
+/-- Get the operator of a term with an operator.
+
+Requires that this term has an operator (see `hasOp`).
+-/
+extern_def!? getOp : Term ω → Except Error (Op ω)
+
+/-- Get the value of a Boolean term as a native Boolean value.
+
+Requires `term` to have sort Bool.
+-/
+extern_def!? getBooleanValue : Term ω → Except Error Bool
+
+/-- Get the string representation of a bit-vector value.
+
+Requires `term` to have a bit-vector sort.
+
+- `base`: `2` for binary, `10` for decimal, and `16` for hexadecimal.
+-/
+extern_def!? getBitVectorValue : Term ω → UInt32 → Except Error String
+
+/-- Get the native integral value of an integral value. -/
+extern_def!? getIntegerValue : Term ω → Except Error Int
+
+/-- Get the native rational value of a real, rational-compatible value. -/
+extern_def!? getRationalValue : Term ω → Except Error Std.Internal.Rat
+
+/-- Get the symbol of this term.
+
+Requires that this term has a symbol (see `hasSymbol`).
+
+The symbol of the term is the string that was provided when constructing it *via*
+`TermManager.mkConst` or `TermManager.mkVar`.
+-/
+extern_def!? getSymbol : Term ω → Except Error String
+
+/-- Get skolem identifier of this term.
+
+Requires `isSkolem`.
+-/
+extern_def!? getSkolemId : (Term ω) → Except Error SkolemId
+
+/-- Get the skolem indices of this term.
+
+Requires `isSkolem`.
+
+Returns the skolem indices of this term. This is a list of terms that the skolem function is indexed
+by. For example, the array diff skolem `SkolemId.ARRAY_DEQ_DIFF` is indexed by two arrays.
+-/
+extern_def!? getSkolemIndices : Term ω → Except Error (Array (Term ω))
+
+instance : GetElem (Term ω) Nat (Term ω) fun t i => i < t.getNumChildren where
+  getElem t i h := t.get ⟨i, h⟩
+
+protected def forIn {β : Type u} [Monad m]
+  (t : Term ω) (b : β) (f : Term ω → β → m (ForInStep β))
+: m β :=
+  let rec loop (i : Nat) (h : i ≤ t.getNumChildren) (b : β) : m β := do
+    match i, h with
+    | 0,   _ => pure b
+    | i+1, h =>
+      have h' : i < t.getNumChildren := Nat.lt_of_lt_of_le (Nat.lt_succ_self i) h
+      have : t.getNumChildren - 1 < t.getNumChildren := Nat.sub_lt (Nat.zero_lt_of_lt h') (by decide)
+      have : t.getNumChildren - 1 - i < t.getNumChildren := Nat.lt_of_le_of_lt (Nat.sub_le (t.getNumChildren - 1) i) this
+      match (← f t[t.getNumChildren - 1 - i] b) with
+      | ForInStep.done b  => pure b
+      | ForInStep.yield b => loop i (Nat.le_of_lt h') b
+  loop t.getNumChildren (Nat.le_refl _) b
+
+instance : ForIn m (Term ω) (Term ω) where
+  forIn := Term.forIn
+
+/-- Get the children of a term. -/
+def getChildren (t : Term ω) : Array (Term ω) := Id.run do
+  let mut cts := #[]
+  for ct in t do
+    cts := cts.push ct
+  cts
+
+/-- Boolean negation. -/
+protected extern_def!? not : (t : Term ω) → Except Error (Term ω)
+
+/-- Boolean and. -/
+protected extern_def!? and : (lft rgt : Term ω) → Except Error (Term ω)
+
+/-- Boolean or. -/
+protected extern_def!? or : (lft rgt : Term ω) → Except Error (Term ω)
+
+/-- Boolean exclusive or. -/
+protected extern_def!? xor : (lft rgt : Term ω) → Except Error (Term ω)
+
+/-- Equality. -/
+protected extern_def!? eq : (lft rgt : Term ω) → Except Error (Term ω)
+
+/-- Boolean implication. -/
+protected extern_def!? imp : (lft rgt : Term ω) → Except Error (Term ω)
+
+/-- If-then-else.
+
+- `cnd`: condition, must be a Boolean term;
+- `thn`: then-branch of some sort `S`;
+- `els`: else-branch of *the same* sort `S`.
+-/
+protected extern_def!? ite : (cnd thn els : Term ω) → Except Error (Term ω)
 
 end Term
 
 
 
-private opaque SolverImpl : NonemptyType.{0}
+namespace Proof
 
-/-- A cvc5 solver. -/
-private def Solver.Raw : Type := SolverImpl.type
+/-- Get the proof rule used by the root step of the root. -/
+extern_def getRule : Proof ω → ProofRule
 
-namespace Solver.Raw
+/-- Get the proof rewrite rule used by the root step of the proof.
 
-instance : Nonempty Solver.Raw := SolverImpl.property
-
-end Solver.Raw
-
-structure Solver (ω : Type) where
-private mk' ::
-  /-- Underlying raw solver. -/
-  private toRaw : Solver.Raw
-  /-- Parser placeholder. -/
-  private parser : IO.Ref (Option Unit)
-
-namespace Solver
-
-/-- Constructor.
-
-Constructs solver instance from a given term manager instance.
-
-- `tm`: The associated term manager.
+Requires that `getRule` does not return `ProofRule.DSL_REWRITE` or `ProofRule.REWRITE`.
 -/
-@[extern "solver_new"]
-private opaque Raw.new : TermManager → Solver.Raw
+extern_def!? getRewriteRule : Proof ω → Except Error ProofRewriteRule
 
-private def ofManager (tm : TermManager) : BaseIO (Solver ω) := do
-  let parser ← IO.mkRef none
-  return {toRaw := Raw.new tm, parser}
+/-- The conclusion of the root step of the proof. -/
+extern_def getResult : Proof ω → Term ω
 
-def new : Env ω (Solver ω) := Env.managerDo (liftM ∘ ofManager)
+/-- The premises of the root step of the proof. -/
+extern_def getChildren : Proof ω → Array (Proof ω)
 
-section variable (solver : Solver ω)
+/-- The arguments of the root step of the proof as a vector of terms.
 
-private def rawSolverDo (f : Solver.Raw → Env ω α) : Env ω α :=
-  f solver.toRaw
+Some of those terms might be strings.
+-/
+extern_def getArguments : Proof ω → Array (Term ω)
 
-private def rawSolverDo? (f : Solver.Raw → Except Error α) : Env ω α :=
-  solver.rawSolverDo (liftM ∘ f)
+/-- Operator overloading for referential equality of two proofs. -/
+protected extern_def beq : Proof ω → Proof ω → Bool
+
+instance : BEq (Proof ω) := ⟨Proof.beq⟩
+
+/-- Hash function for proofs. -/
+protected extern_def hash : Proof ω → UInt64
+
+instance : Hashable (Proof ω) := ⟨Proof.hash⟩
+
+end Proof
+
+
+
+namespace Solver variable (solver : Solver ω)
 
 @[extern "Solver_declareFun"]
 private opaque Raw.declareFun : (solver : Raw)
@@ -802,952 +1378,4 @@ def declareFun (symbol : String)
 : Env ω (Term ω) :=
   solver.toRaw.declareFun symbol sorts sort fresh
 
-end
-
 end Solver
-
-
-
-/-! ## Environment operations -/
-
-
-
-namespace Env
-
-/-- Get the Boolean sort. -/
-@[extern "termManager_getBooleanSort"]
-private opaque getBooleanSort' : TermManager → Srt ω
-
-def getBooleanSort : Env ω (Srt ω) :=
-  Env.managerDo (return getBooleanSort' ·)
-
-end Env
-
-
-
-namespace Srt
-
--- /-- The null sort. -/
--- extern_def null : Unit → Srt ω
-
--- instance : Inhabited (Srt ω) := ⟨null ()⟩
-
--- /-- Comparison for structural equality. -/
--- protected extern_def beq : (Srt ω) → (Srt ω) → Bool
-
--- instance : BEq (Srt ω) := ⟨Srt.beq⟩
-
--- /-- Less than comparison. -/
--- protected extern_def blt : Srt ω → Srt ω → Bool
-
--- /-- Greater than comparison. -/
--- protected extern_def bgt : Srt ω → Srt ω → Bool
-
--- /-- Less than or equal comparison. -/
--- protected extern_def ble : Srt ω → Srt ω → Bool
-
--- /-- Greater than or equal comparison. -/
--- protected extern_def bge : Srt ω → Srt ω → Bool
-
--- /-- Comparison of two sorts. -/
--- protected def compare (s1 s2 : Srt ω) : Ordering :=
---   if s1.beq s2 then .eq
---   else if s1.bgt s2 then .gt
---   else .lt
-
--- instance : Ord (Srt ω) := ⟨Srt.compare⟩
-
--- instance : LT (Srt ω) where
---   lt := (Srt.blt · ·)
-
--- instance : DecidableLT (Srt ω) :=
---   fun s1 s2 => if h : s1.blt s2 then .isTrue h else .isFalse h
-
--- instance : LE (Srt ω) where
---   le := (Srt.ble · ·)
-
--- instance : DecidableLE (Srt ω) :=
---   fun s1 s2 => if h : s1.ble s2 then .isTrue h else .isFalse h
-
--- /-- Hash function for cvc5 sorts. -/
--- protected extern_def hash : Srt ω → UInt64
-
--- instance : Hashable (Srt ω) := ⟨Srt.hash⟩
-
--- /-- Get the kind of this sort. -/
--- extern_def getKind : Srt ω → SortKind
-
--- /-- Determine if this is the null sort (`Srt ω`). -/
--- extern_def isNull : Srt ω → Bool
-
--- /-- Determine if this is the Boolean sort (SMT-LIB: `Bool`). -/
--- extern_def isBoolean : Srt ω → Bool
-
--- /-- Determine if this is the Integer sort (SMT-LIB: `Int`). -/
--- extern_def isInteger : Srt ω → Bool
-
--- /-- Determine if this is the Real sort (SMT-LIB: `Real`). -/
--- extern_def isReal : Srt ω → Bool
-
--- /-- Determine if this is the String sort (SMT-LIB: `String`). -/
--- extern_def isString : Srt ω → Bool
-
--- /-- Determine if this is the regular expression sort (SMT-LIB: `RegLan`). -/
--- extern_def isRegExp : Srt ω → Bool
-
--- /-- Determine if this is the rounding mode sort (SMT-LIB: `RoundingMode`). -/
--- extern_def isRoundingMode : Srt ω → Bool
-
--- /-- Determine if this is a bit-vector sort (SMT-LIB: `(_ BitVec i)`). -/
--- extern_def isBitVector : Srt ω → Bool
-
--- /-- Determine if this is a floating-point sort (SMT-LIB: `(_ FloatingPoint eb sb)`). -/
--- extern_def isFloatingPoint : Srt ω → Bool
-
--- /-- Determine if this is a datatype sort. -/
--- extern_def isDatatype : Srt ω → Bool
-
--- /-- Determine if this is a datatype constructor sort. -/
--- extern_def isDatatypeConstructor : Srt ω → Bool
-
--- /-- Determine if this is a datatype selector sort. -/
--- extern_def isDatatypeSelector : Srt ω → Bool
-
--- /-- Determine if this is a datatype tester sort. -/
--- extern_def isDatatypeTester : Srt ω → Bool
-
--- /-- Determine if this is a datatype updater sort. -/
--- extern_def isDatatypeUpdater : Srt ω → Bool
-
--- /-- Determine if this is a function sort. -/
--- extern_def isFunction : Srt ω → Bool
-
--- /-- Determine if this is a predicate sort.
-
--- A predicate sort is a function sort that maps to the Boolean sort. All predicate sorts are also
--- function sorts.
--- -/
--- extern_def isPredicate : Srt ω → Bool
-
--- /-- Determine if this is a tuple sort. -/
--- extern_def isTuple : Srt ω → Bool
-
--- /-- Determine if this is a nullable sort. -/
--- extern_def isNullable : Srt ω → Bool
-
--- /-- Determine if this is a record sort.
-
--- **Warning**: this function is experimental and may change in future versions.
--- -/
--- extern_def isRecord : Srt ω → Bool
-
--- /-- Determine if this is an array sort. -/
--- extern_def isArray : Srt ω → Bool
-
--- /-- Determine if this is a finite field sort. -/
--- extern_def isFiniteField : Srt ω → Bool
-
--- /-- Determine if this is a Set sort. -/
--- extern_def isSet : Srt ω → Bool
-
--- /-- Determine if this is a Bag sort. -/
--- extern_def isBag : Srt ω → Bool
-
--- /-- Determine if this is a Sequence sort. -/
--- extern_def isSequence : Srt ω → Bool
-
--- /-- Determine if this is an abstract sort. -/
--- extern_def isAbstract : Srt ω → Bool
-
--- /-- Determine if this is an uninterpreted sort. -/
--- extern_def isUninterpretedSort : Srt ω → Bool
-
--- /-- Determine if this is an uninterpreted sort constructor.
-
--- An uninterpreted sort constructor has arity `> 0` and can be instantiated to construct uninterpreted
--- sorts with given sort parameters.
--- -/
--- extern_def isUninterpretedSortConstructor : Srt ω → Bool
-
--- /-- Determine if this is an instantiated (parametric datatype or uninterpreted sort constructor)
--- sort.
-
--- An instantiated sort is a sort that has been constructed from instantiating a sort with sort
--- arguments --- see also `cvc5.Sort.instantiate`.
--- -/
--- extern_def isInstantiated : Srt ω → Bool
-
--- /-- A string representation of this sort. -/
--- protected extern_def toString : Srt ω → String
-
--- /-- Determine if this term has a symbol (a name).
-
--- For example, free constants and variables have symbols.
--- -/
--- extern_def!? hasSymbol : Srt ω → Except Error Bool
-
--- /-- Get the symbol of this sort.
-
--- The symbol of this sort is the string that was provided when constructing it *via* one of
--- `Solver.mkUninterpretedSort`, `Solver.mkUnresolvedSort`, or
--- `Solver.mkUninterpretedSortConstructorSort`.
--- -/
--- extern_def!? getSymbol : Srt ω → Except Error String
-
--- /-- The arity of a function sort. -/
--- extern_def!? getFunctionArity : Srt ω → Except Error Nat
-
--- /-- The domain sorts of a function sort. -/
--- extern_def!? getFunctionDomainSorts : Srt ω → Except Error (Array (Srt ω))
-
--- /-- The codomain sort of a function sort. -/
--- extern_def!? getFunctionCodomainSort : Srt ω → Except Error (Srt ω)
-
--- /-- The array index sort of an array index. -/
--- extern_def!? getArrayIndexSort : Srt ω → Except Error (Srt ω)
-
--- /-- The array element sort of an array index. -/
--- extern_def!? getArrayElementSort : Srt ω → Except Error (Srt ω)
-
--- /-- The element sort of a set sort. -/
--- extern_def!? getSetElementSort : Srt ω → Except Error (Srt ω)
-
--- /-- The element sort of a bag sort. -/
--- extern_def!? getBagElementSort : Srt ω → Except Error (Srt ω)
-
--- /-- The element sort of a sequence sort. -/
--- extern_def!? getSequenceElementSort : Srt ω → Except Error (Srt ω)
-
--- /-- The sort kind of an abstract sort, which denotes the kind of sorts that this abstract sort
--- denotes.
--- -/
--- extern_def!? getAbstractedKind : Srt ω → Except Error SortKind
-
--- /-- The arity of an uninterpreted sort constructor sort. -/
--- extern_def!? getUninterpretedSortConstructorArity : Srt ω → Except Error UInt32
-
--- /-- The bit-width of the bit-vector sort. -/
--- extern_def!? getBitVectorSize : Srt ω → Except Error UInt32
-
--- /-- The size of the finite field sort. -/
--- extern_def!? getFiniteFieldSize : Srt ω → Except Error Nat
-
--- /-- The bit-width of the exponent of the floating-point sort. -/
--- extern_def!? getFloatingPointExponentSize : Srt ω → Except Error UInt32
-
--- /-- The width of the significand of the floating-point sort. -/
--- extern_def!? getFloatingPointSignificandSize : Srt ω → Except Error UInt32
-
--- /-- The length of a tuple sort. -/
--- extern_def!? getTupleLength : Srt ω → Except Error UInt32
-
--- /-- The element sorts of a tuple sort. -/
--- extern_def!? getTupleSorts : Srt ω → Except Error (Array (Srt ω))
-
--- /-- The element sort of a nullable sort. -/
--- extern_def!? getNullableElementSort : Srt ω → Except Error (Srt ω)
-
--- /-- Get the associated uninterpreted sort constructor of an instantiated uninterpreted sort. -/
--- extern_def!? getUninterpretedSortConstructor : Srt ω → Except Error (Srt ω)
-
--- /-- Instantiate a parameterized datatype sort or uninterpreted sort constructor sort.
-
--- Create sort parameters with `TermManager.mkParamSort symbol`.
-
--- - `params` The list of sort parameters to instantiate with.
--- -/
--- extern_def!? instantiate : Srt ω → (params : Array (Srt ω)) → Except Error (Srt ω)
-
--- /-- Simultaneous substitution of Sorts.
-
--- Note that this replacement is applied during a pre-order traversal and only once to the sort. It is not run until fix point. In the case that `sorts` contains duplicates, the replacement earliest in
--- the vector takes priority.
-
--- **Warning:** This function is experimental and may change in future versions.
-
--- - `sorts` The sub-sorts to be substituted within this sort.
--- - `replacements` The sort replacing the substituted sub-sorts.
--- -/
--- extern_def!? substitute
--- : Srt ω → (sorts : Array (Srt ω)) → (replacements : Array (Srt ω)) → Except Error (Srt ω)
-
--- instance : ToString (Srt ω) := ⟨Srt.toString⟩
--- instance : Repr (Srt ω) := ⟨fun self _ => self.toString⟩
-
--- end Srt
-
-
-
--- private opaque OpImpl : NonemptyType.{0}
-
--- /-- A cvc5 operator.
-
--- An operator is a term that represents certain operators, instantiated with its required parameters,
--- *e.g.*, a `Term` of kind `Kind.BITVECTOR_EXTRACT`.
--- -/
--- @[irreducible]
--- def Op : (ω : Type) → Type := fun _ => OpImpl.type
-
--- namespace Op
-
--- private theorem typeDef : Op ω = OpImpl.type :=
---   by unfold Op ; rfl
-
--- private def toImpl : Op ω → OpImpl.type :=
---   by rw [typeDef] ; exact id
-
--- private def ofImpl : OpImpl.type → Op ω :=
---   by rw [typeDef] ; exact id
-
--- instance : Nonempty (Op ω) :=
---   by rw [typeDef] ; exact OpImpl.property
-
--- /-- The null operator. -/
--- extern_def null : Unit → Op ω
-
--- instance : Inhabited Op := ⟨null ()⟩
-
--- /-- Syntactic equality operator. -/
--- protected extern_def beq : Op → Op → Bool
-
--- instance : BEq Op := ⟨Op.beq⟩
-
--- /-- Get the kind of this operator. -/
--- extern_def getKind : Op → Kind
-
--- /-- Determine if this operator is nullary. -/
--- extern_def isNull : Op → Bool
-
--- /-- Determine if this operator is indexed. -/
--- extern_def isIndexed : Op → Bool
-
--- /-- Get the number of indices of this operator. -/
--- extern_def getNumIndices : Op → Nat
-
--- /-- Get the index at position `i` of an indexed operator. -/
--- protected extern_def get : (op : Op) → Fin op.getNumIndices → Term ω
-
--- /-- Get the string representation of this operator. -/
--- protected extern_def toString : Op → String
-
--- instance {ω : outParam Type} : GetElem Op Nat (Term ω) fun op i => i < op.getNumIndices where
---   getElem op i h := op.get ⟨i, h⟩
-
--- instance : ToString Op := ⟨Op.toString⟩
-
--- end Op
-
--- namespace Term
-
--- /-- The null term. -/
--- extern_def null : Unit → Term
-
--- instance : Inhabited Term := ⟨null ()⟩
-
--- /-- Syntactic equality operator. -/
--- protected extern_def beq : Term → Term → Bool
-
--- instance : BEq Term := ⟨Term.beq⟩
-
--- protected extern_def hash : Term → UInt64
-
--- instance : Hashable Term := ⟨Term.hash⟩
-
--- /-- Determine if this term is nullary. -/
--- extern_def isNull : Term → Bool
-
--- /-- Get the kind of this term. -/
--- extern_def getKind : Term → Kind
-
--- /-- Get the sort of this term. -/
--- extern_def getSort : Term → cvc5.Sort
-
--- /-- Determine if this term has an operator. -/
--- extern_def hasOp : Term → Bool
-
--- /-- Determine if this term has a symbol (a name).
-
--- For example, free constants and variables have symbols.
--- -/
--- extern_def hasSymbol : Term → Bool
-
--- /-- Get the id of this term. -/
--- extern_def getId : Term → Nat
-
--- /-- Get the number of children of this term. -/
--- extern_def getNumChildren : Term → Nat
-
--- /-- Is this term a skolem? -/
--- extern_def isSkolem : Term → Bool
-
--- /-- Get the child term of this term at a given index. -/
--- protected extern_def get : (t : Term) → Fin t.getNumChildren → Term
-
--- /-- Get the operator of a term with an operator.
-
--- Requires that this term has an operator (see `hasOp`).
--- -/
--- extern_def!? getOp : Term → Except Error Op
-
--- /-- Get the value of a Boolean term as a native Boolean value.
-
--- Requires `term` to have sort Bool.
--- -/
--- extern_def!? getBooleanValue : Term → Except Error Bool
-
--- /-- Get the string representation of a bit-vector value.
-
--- Requires `term` to have a bit-vector sort.
-
--- - `base`: `2` for binary, `10` for decimal, and `16` for hexadecimal.
--- -/
--- extern_def!? getBitVectorValue : Term → UInt32 → Except Error String
-
--- /-- Get the native integral value of an integral value. -/
--- extern_def!? getIntegerValue : Term → Except Error Int
-
--- /-- Get the native rational value of a real, rational-compatible value. -/
--- extern_def!? getRationalValue : Term → Except Error Std.Internal.Rat
-
--- /-- Get the symbol of this term.
-
--- Requires that this term has a symbol (see `hasSymbol`).
-
--- The symbol of the term is the string that was provided when constructing it *via*
--- `TermManager.mkConst` or `TermManager.mkVar`.
--- -/
--- extern_def!? getSymbol : Term → Except Error String
-
--- /-- Get skolem identifier of this term.
-
--- Requires `isSkolem`.
--- -/
--- extern_def!? getSkolemId : Term → Except Error SkolemId
-
--- /-- Get the skolem indices of this term.
-
--- Requires `isSkolem`.
-
--- Returns the skolem indices of this term. This is a list of terms that the skolem function is indexed
--- by. For example, the array diff skolem `SkolemId.ARRAY_DEQ_DIFF` is indexed by two arrays.
--- -/
--- extern_def!? getSkolemIndices : Term → Except Error (Array Term)
-
--- instance : GetElem Term Nat Term fun t i => i < t.getNumChildren where
---   getElem t i h := t.get ⟨i, h⟩
-
--- protected def forIn {β : Type u} [Monad m] (t : Term) (b : β) (f : Term → β → m (ForInStep β)) : m β :=
---   let rec loop (i : Nat) (h : i ≤ t.getNumChildren) (b : β) : m β := do
---     match i, h with
---     | 0,   _ => pure b
---     | i+1, h =>
---       have h' : i < t.getNumChildren := Nat.lt_of_lt_of_le (Nat.lt_succ_self i) h
---       have : t.getNumChildren - 1 < t.getNumChildren := Nat.sub_lt (Nat.zero_lt_of_lt h') (by decide)
---       have : t.getNumChildren - 1 - i < t.getNumChildren := Nat.lt_of_le_of_lt (Nat.sub_le (t.getNumChildren - 1) i) this
---       match (← f t[t.getNumChildren - 1 - i] b) with
---       | ForInStep.done b  => pure b
---       | ForInStep.yield b => loop i (Nat.le_of_lt h') b
---   loop t.getNumChildren (Nat.le_refl _) b
-
--- instance : ForIn m Term Term where
---   forIn := Term.forIn
-
--- /-- Get the children of a term. -/
--- def getChildren (t : Term) : Array Term := Id.run do
---   let mut cts := #[]
---   for ct in t do
---     cts := cts.push ct
---   cts
-
--- /-- Boolean negation. -/
--- protected extern_def!? not : (t : Term) → Except Error Term
-
--- /-- Boolean and. -/
--- protected extern_def!? and : (lft rgt : Term) → Except Error Term
-
--- /-- Boolean or. -/
--- protected extern_def!? or : (lft rgt : Term) → Except Error Term
-
--- /-- Boolean exclusive or. -/
--- protected extern_def!? xor : (lft rgt : Term) → Except Error Term
-
--- /-- Equality. -/
--- protected extern_def!? eq : (lft rgt : Term) → Except Error Term
-
--- /-- Boolean implication. -/
--- protected extern_def!? imp : (lft rgt : Term) → Except Error Term
-
--- /-- If-then-else.
-
--- - `cnd`: condition, must be a Boolean term;
--- - `thn`: then-branch of some sort `S`;
--- - `els`: else-branch of *the same* sort `S`.
--- -/
--- protected extern_def!? ite : (cnd thn els : Term) → Except Error Term
-
--- /-- A string representation of this term. -/
--- protected extern_def toString : Term → String
-
--- instance : ToString Term := ⟨Term.toString⟩
-
--- end Term
-
--- namespace Proof
-
--- /-- The null proof. -/
--- extern_def null : Unit → Proof
-
--- instance : Inhabited Proof := ⟨null ()⟩
-
--- /-- Get the proof rule used by the root step of the root. -/
--- extern_def getRule : Proof → ProofRule
-
--- /-- Get the proof rewrite rule used by the root step of the proof.
-
--- Requires that `getRule` does not return `ProofRule.DSL_REWRITE` or `ProofRule.REWRITE`.
--- -/
--- extern_def!? getRewriteRule : Proof → Except Error ProofRewriteRule
-
--- /-- The conclusion of the root step of the proof. -/
--- extern_def getResult : Proof → Term
-
--- /-- The premises of the root step of the proof. -/
--- extern_def getChildren : Proof → Array Proof
-
--- /-- The arguments of the root step of the proof as a vector of terms.
-
--- Some of those terms might be strings.
--- -/
--- extern_def getArguments : Proof → Array Term
-
--- /-- Operator overloading for referential equality of two proofs. -/
--- protected extern_def beq : Proof → Proof → Bool
-
--- instance : BEq Proof := ⟨Proof.beq⟩
-
--- /-- Hash function for proofs. -/
--- protected extern_def hash : Proof → UInt64
-
--- instance : Hashable Proof := ⟨Proof.hash⟩
-
--- end Proof
-
--- namespace TermManager
-
--- /-- Constructor. -/
--- extern_def new : BaseIO TermManager
-
--- /-- Get the Boolean sort. -/
--- extern_def getBooleanSort : TermManager → cvc5.Sort
-
--- /-- Get the Integer sort. -/
--- extern_def getIntegerSort : TermManager → cvc5.Sort
-
--- /-- Get the Real sort. -/
--- extern_def getRealSort : TermManager → cvc5.Sort
-
--- /-- Get the regular expression sort. -/
--- extern_def getRegExpSort : TermManager → cvc5.Sort
-
--- /-- Get the rounding mode sort. -/
--- extern_def getRoundingModeSort : TermManager → cvc5.Sort
-
--- /-- Get the string sort. -/
--- extern_def getStringSort : TermManager → cvc5.Sort
-
--- /-- Create an array sort.
-
--- - `indexSort` The array index sort.
--- - `elemSort` The array element sort.
--- -/
--- extern_def!? mkArraySort : TermManager → (indexSort elemSort : cvc5.Sort) → Except Error cvc5.Sort
-
--- /-- Create a bit-vector sort.
-
--- - `size` The bit-width of the bit-vector sort.
--- -/
--- extern_def!? mkBitVectorSort : TermManager → (size : UInt32) → Except Error cvc5.Sort
-
--- /-- Create a floating-point sort.
-
--- - `exp` The bit-width of the exponent of the floating-point sort.
--- - `sig` The bit-width of the significand of the floating-point sort.
--- -/
--- extern_def!? mkFloatingPointSort : TermManager → (exp sig : UInt32) → Except Error cvc5.Sort
-
--- /-- Create a finite-field sort from a given string of base n.
-
--- - `size` The modulus of the field. Must be a prime.
--- -/
--- private extern_def mkFiniteFieldSortFromString : TermManager → (size : String) → (base : UInt32 := 10) → Except Error cvc5.Sort
-
--- @[inherit_doc mkFiniteFieldSortFromString]
--- abbrev mkFiniteFieldSort (tm : TermManager) : (size : Nat) → Except Error cvc5.Sort :=
---   (tm.mkFiniteFieldSortFromString · 10) ∘ toString
--- @[inherit_doc mkFiniteFieldSortFromString]
--- abbrev mkFiniteFieldSort! (tm : TermManager) : (size : Nat) → cvc5.Sort :=
---   Error.unwrap! ∘ (tm.mkFiniteFieldSortFromString · 10) ∘ toString
--- @[inherit_doc mkFiniteFieldSortFromString]
--- abbrev mkFiniteFieldSort? (tm : TermManager) : (size : Nat) → Option cvc5.Sort :=
---   Except.toOption ∘ (tm.mkFiniteFieldSortFromString · 10) ∘ toString
-
--- /-- Create function sort.
-
--- - `sorts` The sort of the function arguments.
--- - `codomain` The sort of the function return value.
--- -/
--- extern_def!? mkFunctionSort
--- : TermManager → (sorts : Array cvc5.Sort) → (codomain : cvc5.Sort) → Except Error cvc5.Sort
-
--- /-- Create a predicate sort.
-
--- This is equivalent to calling `mkFunctionSort` with Boolean sort as the codomain.
-
--- - `sorts` The list of sorts of the predicate.
--- -/
--- extern_def!? mkPredicateSort : TermManager → (sorts : Array cvc5.Sort) → Except Error cvc5.Sort
-
--- /-- Create a tuple sort.
-
--- - `sorts` The sorts of the elements of the tuple.
--- -/
--- extern_def!? mkTupleSort : TermManager → (sorts : Array cvc5.Sort) → Except Error cvc5.Sort
-
--- /-- Create an uninterpreted sort constructor sort.
-
--- An uninterpreted sort constructor is an uninterpreted sort with arity > 0.
-
--- - `arity` The arity of the sort (must be > 0).
--- - `symbol` The symbol of the sort.
--- -/
--- extern_def!? mkUninterpretedSortConstructorSort
--- : TermManager → (arity : Nat) → (symbol : String) → Except Error cvc5.Sort
-
--- /-- Create a set parameter.
-
--- - `elemSort` The sort of the set elements.
--- -/
--- extern_def!? mkSetSort : TermManager → (sort : cvc5.Sort) → Except Error cvc5.Sort
-
--- /-- Create a set parameter.
-
--- - `elemSort` The sort of the set elements.
--- -/
--- extern_def!? mkBagSort : TermManager → (sort : cvc5.Sort) → Except Error cvc5.Sort
-
--- /-- Create a set parameter.
-
--- - `elemSort` The sort of the set elements.
--- -/
--- extern_def!? mkSequenceSort : TermManager → (sort : cvc5.Sort) → Except Error cvc5.Sort
-
--- /-- Create an abstract sort. An abstract sort represents a sort for a given kind whose parameters
--- and arguments are unspecified.
-
--- The kind `k` must be the kind of a sort that can be abstracted, *i.e.* a sort that has indices or
--- arguments sorts. For example, `SortKind.ARRAY_SORT` and `SortKind.BITVECTOR_SORT` can be passed as
--- the kind `k` to this function, while `SortKind.INTEGER_SORT` and `SortKind.STRING_SORT` cannot.
-
--- **NB:** Providing the kind `SortKind.ABSTRACT_SORT` as an argument to this function returns the
--- (fully) unspecified sort, denoted `?`.
-
--- **NB:** Providing a kind `k` that has no indices and a fixed arity of argument sorts will return the
--- sort of kind `k` whose arguments are the unspecified sort. For example, `mkAbstractSort
--- SortKind.ARRAY_SORT` will return the sort `(ARRAY_SORT ? ?)` instead of the abstract sort whose
--- abstract kind is `SortKind.ARRAY_SORT`.
--- -/
--- extern_def!? mkAbstractSort : TermManager → (k : SortKind) → Except Error cvc5.Sort
-
--- /-- Create an uninterpreted sort.
-
--- - `symbol` The name of the sort.
--- -/
--- extern_def mkUninterpretedSort : TermManager → (symbol : String) → cvc5.Sort
-
--- /-- Create a nullable sort.
-
--- - `sort` The sort of the element of the nullable.
--- -/
--- extern_def!? mkNullableSort : TermManager → (sort : cvc5.Sort) → Except Error cvc5.Sort
-
--- /-- Create a sort parameter.
-
--- - `symbol` The name of the sort.
-
--- **Warning**: This function is experimental and may change in future versions.
--- -/
--- extern_def mkParamSort : TermManager → (symbol : String) → cvc5.Sort
-
--- /-- Create a Boolean constant.
-
--- - `b`: The Boolean constant.
--- -/
--- extern_def mkBoolean : TermManager → (b : Bool) → Term
-
--- /-- Create an integer-value term.
-
--- - `s`: the string representation of the constant, may represent an integer such as (`"123"`).
--- -/
--- private extern_def mkIntegerFromString : TermManager → (s : String) → Except Error Term
--- with
---   /-- Create an integer-value term. -/
---   mkInteger (tm : TermManager) : Int → Term :=
---     Error.unwrap! ∘ tm.mkIntegerFromString ∘ toString
-
--- /-- Create a real-value term.
-
--- - `s`: the string representation of the constant, may represent an integer (`"123"`) or a real
---   constant (`"12.34"`, `"12/34"`).
--- -/
--- private extern_def mkRealFromString : TermManager → (s : String) → Except Error Term
--- with
---   /-- Create a real-value term from a `Std.Internal.Rat`. -/
---   mkRealOfRat (tm : TermManager) (rat : Std.Internal.Rat) : Term :=
---     tm.mkRealFromString s!"{rat.num}/{rat.den}" |> Error.unwrap!
---   /-- Create a real-value term from numerator/denominator `Int`-s. -/
---   mkReal (tm : TermManager)
---     (num : Int) (den : Int := 1) (den_ne_0 : den ≠ 0 := by simp <;> omega)
---   : Term :=
---     let (num, den) :=
---       match h : den with
---       | .ofNat 0 => by contradiction
---       | .ofNat den => (num, den)
---       | .negSucc denMinus1 => (-num, denMinus1.succ)
---     tm.mkRealOfRat <| Std.Internal.mkRat num den
-
--- /-- Create operator of Kind:
-
--- - `Kind.BITVECTOR_EXTRACT`
--- - `Kind.BITVECTOR_REPEAT`
--- - `Kind.BITVECTOR_ROTATE_LEFT`
--- - `Kind.BITVECTOR_ROTATE_RIGHT`
--- - `Kind.BITVECTOR_SIGN_EXTEND`
--- - `Kind.BITVECTOR_ZERO_EXTEND`
--- - `Kind.DIVISIBLE`
--- - `Kind.FLOATINGPOINT_TO_FP_FROM_FP`
--- - `Kind.FLOATINGPOINT_TO_FP_FROM_IEEE_BV`
--- - `Kind.FLOATINGPOINT_TO_FP_FROM_REAL`
--- - `Kind.FLOATINGPOINT_TO_FP_FROM_SBV`
--- - `Kind.FLOATINGPOINT_TO_FP_FROM_UBV`
--- - `Kind.FLOATINGPOINT_TO_SBV`
--- - `Kind.FLOATINGPOINT_TO_UBV`
--- - `Kind.INT_TO_BITVECTOR`
--- - `Kind.TUPLE_PROJECT`
-
--- See `cvc5.Kind` for a description of the parameters.
-
--- - `kind` The kind of the operator.
--- - `args` The arguments (indices) of the operator.
-
--- If `args` is empty, the `Op` simply wraps the `cvc5.Kind`. The `Kind` can be used in
--- `Solver.mkTerm` directly without creating an `Op` first.
--- -/
--- extern_def!? mkOpOfIndices : TermManager → (kind : Kind) → (args : Array Nat := #[]) → Except Error Op
-
--- @[inherit_doc mkOpOfIndices]
--- abbrev mkOp := @mkOpOfIndices
--- @[inherit_doc mkOpOfIndices!]
--- abbrev mkOp! := @mkOpOfIndices!
--- @[inherit_doc mkOpOfIndices?]
--- abbrev mkOp? := @mkOpOfIndices?
-
--- /-- Create operator of kind:
-
--- - `Kind.DIVISIBLE` (to support arbitrary precision integers)
-
--- See `cvc5.Kind` for a description of the parameters.
-
--- - `kind` The kind of the operator.
--- - `arg` The string argument to this operator.
--- -/
--- extern_def!? mkOpOfString : TermManager → (kind : Kind) → (arg : String) → Except Error Op
-
--- /-- Create n-ary term of given kind.
-
--- - `kind` The kind of the term.
--- - `children` The children of the term.
--- -/
--- extern_def!? mkTerm : TermManager → (kind : Kind) → (children : Array Term := #[]) → Except Error Term
-
--- /-- Create n-ary term of given kind from a given operator.
-
--- Create operators with `mkOp`.
-
--- - `op` The operator.
--- - `children` The children of the term.
--- -/
--- extern_def!? mkTermOfOp : TermManager → (op : Op) → (children : Array Term := #[]) → Except Error Term
-
--- /-- **THIS FUNCTION MUST NOT BE EXPOSED.**
-
--- **It produces a different (fresh) term every time it's called which is really bad for purity.**
-
--- Create a free constant.
-
--- Note that the returned term is always fresh, even if the same arguments were provided on a
--- previous call to `mkConst`.
-
--- - `sort` The sort of the constant.
--- - `symbol` The name of the constant (optional).
--- -/
--- private
--- def mkConst (_ : TermManager) (_ : cvc5.Sort) (_ : String := "") : Term :=
---   panic! "illegal call to `cvc5.TermManager.mkConst"
-
--- end TermManager
-
--- namespace Solver
-
--- variable [Monad m]
-
--- /-- Only used by FFI to wrap *success* results. -/
--- @[export solver_val]
--- private def val (a : α) : SolverT m α := pure a
-
--- /-- Only used by FFI to wrap errors. -/
--- @[export solver_err]
--- private def err (e : Error) : SolverT m α := throw e
-
--- /-- Only used by FFI to wrap cvc5 errors. -/
--- @[export solver_errOfString]
--- private def errorOfString (msg : String) : SolverT m α := throw (.error msg)
-
--- /-- Constructor.
-
--- Constructs solver instance from a given term manager instance.
-
--- - `tm`: The associated term manager.
--- -/
--- private extern_def new : TermManager → Solver
-
--- /-- Get a string representation of the version of this solver. -/
--- extern_def getVersion : SolverT m String
-
--- /-- Set option.
-
--- - `option`: The option name.
--- - `value`: The option value.
--- -/
--- extern_def setOption (option value : String) : SolverT m Unit
-
--- /-- Remove all assertions. -/
--- extern_def resetAssertions : SolverT m Unit
-
--- /-- Set logic.
-
--- - `logic`: The logic to set.
--- -/
--- extern_def setLogic : (logic : String) → SolverT m Unit
-
--- /-- Simplify a term or formula based on rewriting and (optionally) applying substitutions for
--- solved variables.
-
--- If `applySubs` is true, then for example, if `(= x 0)` was asserted to this solver, this function
--- may replace occurrences of `x` with `0`.
-
--- - `t` The term to simplify.
--- - `applySubs` True to apply substitutions for solved variables.
--- -/
--- extern_def simplify : (term : Term) → (applySubs : Bool := false) → SolverT m Term
-
--- /--
--- Declare n-ary function symbol.
-
--- SMT-LIB:
-
--- \verbatim embed:rst:leading-asterisk
---  .. code:: smtlib
-
---      (declare-fun <symbol> ( <sort>* ) <sort>)
---  \endverbatim
-
--- - `symbol`: The name of the function.
--- - `sorts`: The sorts of the parameters to this function.
--- - `sort`: The sort of the return value of this function.
--- - `fresh`: If true, then this method always returns a new Term. Otherwise, this method will always
---   return the same Term for each call with the given sorts and symbol where fresh is false.
--- -/
--- extern_def declareFun (symbol : String) (sorts : Array cvc5.Sort) (sort : cvc5.Sort) (fresh := true) : SolverT m Term
-
--- /-- Assert a formula.
-
--- - `term`: The formula to assert.
--- -/
--- extern_def assertFormula : Term → SolverT m Unit
-
--- /-- Check satisfiability. -/
--- extern_def checkSat : SolverT m Result
-
--- /-- Check satisfiability assuming the given formulas.
-
--- - `assumptions`: The formulas to assume.
--- -/
--- extern_def checkSatAssuming : (assumptions : Array Term) → SolverT m Result
-
--- /-- Get a proof associated with the most recent call to `checkSat`.
-
--- Requires to enable option `produce-proofs`.
--- -/
--- extern_def getProof : SolverT m (Array Proof)
-
--- /--
--- Get the values of the given term in the current model.
-
--- SMT-LIB:
-
--- \verbatim embed:rst:leading-asterisk
--- .. code:: smtlib
-
---     (get-value ( <term>* ))
--- \endverbatim
-
--- - `terms`: The term for which the value is queried.
--- -/
--- extern_def getValue (term : Term) : SolverT m Term
-
--- /--
--- Get the values of the given terms in the current model.
-
--- SMT-LIB:
-
--- \verbatim embed:rst:leading-asterisk
--- .. code:: smtlib
-
---     (get-value ( <term>* ))
--- \endverbatim
-
--- - `terms`: The terms for which the values are queried.
--- -/
--- extern_def getValues (terms : Array Term) : SolverT m (Array Term)
-
--- /-- Prints a proof as a string in a selected proof format mode.
-
--- Other aspects of printing are taken from the solver options.
-
--- - `proof`: A proof, usually obtained from `getProof`.
--- -/
--- extern_def proofToString : Proof → SolverT m String
-
--- /-- Parse a string containing SMT-LIB commands.
-
--- Commands that produce a result such as `(check-sat)`, `(get-model)`, ... are executed but the
--- results are ignored.
--- -/
--- extern_def parseCommands : String → SolverT m Unit
-
--- /-- Run a `query` given a term manager `tm`. -/
--- def run (tm : TermManager) (query : SolverT m α) : m (Except Error α) :=
---   return match ← ExceptT.run query (new tm) with
---   | (.ok x, _) => .ok x
---   | (.error e, _) => .error e
-
--- /-- Run a `query` given a term manager `tm`. -/
--- def run! [Inhabited α] (tm : TermManager) (query : SolverT m α) : m α := do
---   match ← ExceptT.run query (new tm) with
---   | (.ok x, _) => return x
---   | (.error e, _) => do
---     panic! s!"{e}"
-
--- end Solver
-
--- end cvc5
