cvcTests/Test.lean
@@ -2,21 +2,28 @@ import cvc5
 
 
 
-namespace Cvc5.Test
+namespace Test
 
 /-- info: bool = `Bool` -/
-#guard_msgs in #eval Env.runIO do
-  let bool ← Env.getBooleanSort
+#guard_msgs in #eval Cvc5.runIO do
+  let bool ← Cvc5.getBooleanSort
   println! "bool = `{bool}`"
 
 /-- error: [error] not a function sort: Bool -/
-#guard_msgs in #eval Env.runIO do
-  let bool ← Env.getBooleanSort
+#guard_msgs in #eval Cvc5.runIO do
+  let bool ← Cvc5.getBooleanSort
   let _sorts ← bool.getFunctionDomainSorts
 
+/-- info: Bool.substitute [Bool → Int] = Int -/
+#guard_msgs in #eval Cvc5.runIO do
+  let bool ← Cvc5.getBooleanSort
+  let int ← Cvc5.getIntegerSort
+  let sub ← bool.substitute #[bool] #[int]
+  println! "{bool}.substitute [{bool} → {int}] = {sub}"
+
 /-- info: x = `x` -/
-#guard_msgs in #eval Env.runIO do
-  let bool ← Env.getBooleanSort
-  let solver ← Solver.new
+#guard_msgs in #eval Cvc5.runIO do
+  let bool ← Cvc5.getBooleanSort
+  let solver ← Cvc5.Solver.new
   let x ← solver.declareFun "x" #[] bool
   println! "x = `{x}`"
